Logic/Logic/Sequent.lean
@@ -1,75 +1,139 @@
 import Logic.Logic.System
 
 /-!
-# Sequent calculus and variants
+# TwosidedCalc calculus and variants
 
 -/
 
 namespace LO
 
-class Sequent {F : outParam Type*} (L R : outParam Type*) [Collection F L] [Collection F R] (S : Type*) where
-  Seq : S → L → R → Type*
+class TwosidedCalc {F : outParam Type*} (L R : outParam Type*) [Collection F L] [Precollection F R] (C : Type*) where
+  Sqt : C → L → R → Type*
 
-notation:45 Δ:45 " ⟹[" 𝓢 "] " Γ:46 => Sequent.Seq 𝓢 Δ Γ
+notation:45 Δ:45 " ⟹[" 𝓒 "] " Γ:46 => TwosidedCalc.Sqt 𝓒 Δ Γ
 
-namespace Sequent
+namespace TwosidedCalc
 
-variable {F : Type*} {L R : Type*} [Collection F L] [Collection F R] {S : Type*} [Sequent L R S]
+variable {F : Type*} {L R : Type*} [Collection F L] [Precollection F R] {C : Type*} [TwosidedCalc L R C]
 
 scoped infixr:60 " ∷ " => Cons.cons
 
-abbrev SingleConseq (𝓢 : S) (Γ : L) (A : F) := Γ ⟹[𝓢] {A}
+scoped infixr:50 " ⊹ " => Tie.tie
 
-notation:45 Γ:45 " ⟹[" 𝓢 "]. " A:46 => SingleConseq 𝓢 Γ A
+abbrev SingleConseq (𝓒 : C) (Γ : L) (A : F) := Γ ⟹[𝓒] {A}
 
-abbrev SingleAntecedent (𝓢 : S) (A : F) (Γ : R) := {A} ⟹[𝓢] Γ
+notation:45 Γ:45 " ⟹[" 𝓒 "]. " A:46 => SingleConseq 𝓒 Γ A
 
-notation:45 A:45 " .⟹[" 𝓢 "] " Γ:46 => SingleAntecedent 𝓢 A Γ
+abbrev SingleAntecedent (𝓒 : C) (A : F) (Γ : R) := {A} ⟹[𝓒] Γ
 
-abbrev SingleAntecedentConseq (𝓢 : S) (A B : F) := {A} ⟹[𝓢] {B}
+notation:45 A:45 " .⟹[" 𝓒 "] " Γ:46 => SingleAntecedent 𝓒 A Γ
 
-notation:45 A:45 " .⟹[" 𝓢 "]. " B:46 => SingleAntecedentConseq 𝓢 A B
+abbrev SingleAntecedentConseq (𝓒 : C) (A B : F) := {A} ⟹[𝓒] {B}
 
-class Closed (𝓢 : S) where
-  closed {Γ Δ} (A : F) : A ∈ Γ → A ∈ Δ → Γ ⟹[𝓢] Δ
+notation:45 A:45 " .⟹[" 𝓒 "]. " B:46 => SingleAntecedentConseq 𝓒 A B
 
-class IRefl (𝓢 : S) where
-  irefl (A) : A .⟹[𝓢]. A
+class Id (𝓒 : C) where
+  id (A) : A .⟹[𝓒]. A
 
-class ICut (𝓢 : S) where
-  icut {Γ A Λ} : Γ ⟹[𝓢]. A → A .⟹[𝓢] Λ → Γ ⟹[𝓢] Λ
+class ICut (𝓒 : C) where
+  icut {Γ A Δ} : Γ ⟹[𝓒]. A → A ∷ Δ ⟹[𝓒] Λ → Γ ⟹[𝓒] Λ
 
-class Weakening (𝓢 : S) where
-  wk {Γ₁ Γ₂ Δ₁ Δ₂} : Γ₁ ⊆ Γ₂ → Δ₁ ⊆ Δ₂ → Γ₁ ⟹[𝓢] Δ₁ → Γ₂ ⟹[𝓢] Δ₂
+class Weakening (𝓒 : C) where
+  wk {Γ₁ Γ₂ Δ₁ Δ₂} : Γ₁ ⊆ Γ₂ → Δ₁ ⊆ Δ₂ → Γ₁ ⟹[𝓒] Δ₁ → Γ₂ ⟹[𝓒] Δ₂
 
-variable [LogicalConnective F] [Cons F L]
+export Weakening (wk)
 
-class LJ (𝓢 : S) extends IRefl 𝓢, Weakening 𝓢 where
-  verum (Γ)            : Γ ⟹[𝓢]. ⊤
-  falsum               : ⊥ .⟹[𝓢] ∅
-  negLeft {Γ A}        : Γ ⟹[𝓢]. A → ~A ∷ Γ ⟹[𝓢] ∅
-  negRight {Γ A}       : A ∷ Γ ⟹[𝓢]. ⊥ → Γ ⟹[𝓢]. ~A
-  andLeft₁ {Γ A B}     : A ∷ Γ ⟹[𝓢]. C → A ⋏ B ∷ Γ ⟹[𝓢] Δ
-  andLeft₂ {Γ A B}     : B ∷ Γ ⟹[𝓢]. C → A ⋏ B ∷ Γ ⟹[𝓢] Δ
-  andRight {Γ A B}     : Γ ⟹[𝓢]. A → Γ ⟹[𝓢]. B → Γ ⟹[𝓢]. A ⋏ B
-  orLeft {Γ A B}       : A ∷ Γ ⟹[𝓢]. C → B ∷ Γ ⟹[𝓢]. C → A ⋎ B ∷ Γ ⟹[𝓢]. C
-  orRight₁ {Γ A B}     : Γ ⟹[𝓢]. A → Γ ⟹[𝓢]. A ⋎ B
-  orRight₂ {Γ A B}     : Γ ⟹[𝓢]. B → Γ ⟹[𝓢]. A ⋎ B
-  implyLeft {Γ A B C}  : Γ ⟹[𝓢]. A → B ∷ Γ ⟹[𝓢]. C → (A ⟶ B) ∷ Γ ⟹[𝓢]. C
-  implyRight {Γ A B}   : A ∷ Γ ⟹[𝓢]. B → Γ ⟹[𝓢]. (A ⟶ B)
+section
 
-variable [Cons F R]
+variable {𝓒 : C} [Weakening 𝓒]
 
-class LK (𝓢 : S) extends IRefl 𝓢, Weakening 𝓢 where
-  verum (Γ Δ)          : Γ ⟹[𝓢] ⊤ ∷ Δ
-  falsum (Γ Δ)         : ⊥ ∷ Γ ⟹[𝓢] Δ
-  negLeft {A Γ Δ}      : Γ ⟹[𝓢] A ∷ Δ → ~A ∷ Γ ⟹[𝓢] Δ
-  negRight {A Γ Δ}     : A ∷ Γ ⟹[𝓢] Δ → Γ ⟹[𝓢] ~A ∷ Δ
-  andLeft {A B Γ Δ}    : A ∷ B ∷ Γ ⟹[𝓢] Δ → A ⋏ B ∷ Γ ⟹[𝓢] Δ
-  andRight {A B Γ Δ}   : Γ ⟹[𝓢] A ∷ Δ → Γ ⟹[𝓢] B ∷ Δ → Γ ⟹[𝓢] A ⋏ B ∷ Δ
-  orLeft {A B Γ Δ}     : A ∷ Γ ⟹[𝓢] Δ → B ∷ Γ ⟹[𝓢] Δ → A ⋎ B ∷ Γ ⟹[𝓢] Δ
-  orRight {A B Γ Δ}    : Γ ⟹[𝓢] A ∷ B ∷ Δ → Γ ⟹[𝓢] A ⋎ B ∷ Δ
-  implyLeft {A B Γ Δ}  : Γ ⟹[𝓢] A ∷ Δ → B ∷ Γ ⟹[𝓢] Δ → (A ⟶ B) ∷ Γ ⟹[𝓢] Δ
-  implyRight {A B Γ Δ} : A ∷ Γ ⟹[𝓢] B ∷ Δ → Γ ⟹[𝓢] (A ⟶ B) ∷ Δ
+def wkL {Γ₁ Γ₂ Δ} (h : Γ₁ ⊆ Γ₂) : Γ₁ ⟹[𝓒] Δ → Γ₂ ⟹[𝓒] Δ := wk h (by rfl)
 
-end Sequent
+def wkR {Γ Δ₁ Δ₂} (h : Δ₁ ⊆ Δ₂) : Γ ⟹[𝓒] Δ₁ → Γ ⟹[𝓒] Δ₂ := wk (by rfl) h
+
+def closed [Id 𝓒] {Γ Δ} (A : F) : A ∈ Γ → A ∈ Δ → Γ ⟹[𝓒] Δ := fun hΓ hΔ ↦ wk (by simpa) (by simpa) (Id.id A)
+
+end
+
+variable [LogicalConnective F]
+
+class LJ (𝓒 : C) extends Id 𝓒, Weakening 𝓒 where
+  verum (Γ)            : Γ ⟹[𝓒]. ⊤
+  falsum               : ⊥ .⟹[𝓒] ∅
+  negLeft {Γ A}        : Γ ⟹[𝓒]. A → ~A ∷ Γ ⟹[𝓒] ∅
+  negRight {Γ A}       : A ∷ Γ ⟹[𝓒] ∅ → Γ ⟹[𝓒]. ~A
+  andLeft₁ {Γ A B C}   : A ∷ Γ ⟹[𝓒]. C → A ⋏ B ∷ Γ ⟹[𝓒]. C
+  andLeft₂ {Γ A B C}   : B ∷ Γ ⟹[𝓒]. C → A ⋏ B ∷ Γ ⟹[𝓒]. C
+  andRight {Γ A B}     : Γ ⟹[𝓒]. A → Γ ⟹[𝓒]. B → Γ ⟹[𝓒]. A ⋏ B
+  orLeft {Γ A B C}     : A ∷ Γ ⟹[𝓒]. C → B ∷ Γ ⟹[𝓒]. C → A ⋎ B ∷ Γ ⟹[𝓒]. C
+  orRight₁ {Γ A B}     : Γ ⟹[𝓒]. A → Γ ⟹[𝓒]. A ⋎ B
+  orRight₂ {Γ A B}     : Γ ⟹[𝓒]. B → Γ ⟹[𝓒]. A ⋎ B
+  implyLeft {Γ A B C}  : Γ ⟹[𝓒]. A → B ∷ Γ ⟹[𝓒]. C → (A ⟶ B) ∷ Γ ⟹[𝓒]. C
+  implyRight {Γ A B}   : A ∷ Γ ⟹[𝓒]. B → Γ ⟹[𝓒]. (A ⟶ B)
+
+section LJ
+
+variable {𝓒 : C} [LJ 𝓒]
+
+def LJ.verum' (h : ⊤ ∈ Δ) : Γ ⟹[𝓒] Δ := wkR (by simp[h]) (LJ.verum Γ)
+
+-- def ICut.cut' [ICut 𝓒] {Γ Δ : L} (d₁ : Γ ⟹[𝓒]. A) (d₂ : A ∷ Δ ⟹[𝓒]. B) : Γ ∷+ Δ ⟹[𝓒]. B := by {  }
+
+end LJ
+
+end TwosidedCalc
+
+namespace TwosidedCalc
+
+variable {F : Type*} {L : Type*} [Collection F L] {C : Type*} [TwosidedCalc L L C] [LogicalConnective F]
+
+class Cut (𝓒 : C) where
+  cut {Γ Δ Λ} : Γ ⟹[𝓒] Δ → Δ ⟹[𝓒] Λ → Γ ⟹[𝓒] Λ
+
+class LK (𝓒 : C) extends Id 𝓒, Weakening 𝓒 where
+  verum (Γ Δ)          : Γ ⟹[𝓒] ⊤ ∷ Δ
+  falsum (Γ Δ)         : ⊥ ∷ Γ ⟹[𝓒] Δ
+  negLeft {A Γ Δ}      : Γ ⟹[𝓒] A ∷ Δ → ~A ∷ Γ ⟹[𝓒] Δ
+  negRight {A Γ Δ}     : A ∷ Γ ⟹[𝓒] Δ → Γ ⟹[𝓒] ~A ∷ Δ
+  andLeft {A B Γ Δ}    : A ∷ B ∷ Γ ⟹[𝓒] Δ → A ⋏ B ∷ Γ ⟹[𝓒] Δ
+  andRight {A B Γ Δ}   : Γ ⟹[𝓒] A ∷ Δ → Γ ⟹[𝓒] B ∷ Δ → Γ ⟹[𝓒] A ⋏ B ∷ Δ
+  orLeft {A B Γ Δ}     : A ∷ Γ ⟹[𝓒] Δ → B ∷ Γ ⟹[𝓒] Δ → A ⋎ B ∷ Γ ⟹[𝓒] Δ
+  orRight {A B Γ Δ}    : Γ ⟹[𝓒] A ∷ B ∷ Δ → Γ ⟹[𝓒] A ⋎ B ∷ Δ
+  implyLeft {A B Γ Δ}  : Γ ⟹[𝓒] A ∷ Δ → B ∷ Γ ⟹[𝓒] Δ → (A ⟶ B) ∷ Γ ⟹[𝓒] Δ
+  implyRight {A B Γ Δ} : A ∷ Γ ⟹[𝓒] B ∷ Δ → Γ ⟹[𝓒] (A ⟶ B) ∷ Δ
+
+variable {𝓒 : C}
+
+section
+
+variable [Weakening 𝓒]
+
+def ofSingleton {Γ A} (d : Γ ⟹[𝓒]. A) : Γ ⟹[𝓒] A ∷ ∅ := wkR (Precollection.subset_iff.mpr <| by simp) d
+
+def ofCons {Γ A} (d : Γ ⟹[𝓒] A ∷ ∅) : Γ ⟹[𝓒]. A := wkR (Precollection.subset_iff.mpr <| by simp) d
+
+end
+
+section LK
+
+variable (𝓒) [LK 𝓒]
+
+instance : LJ 𝓒 where
+  verum (Γ) := ofCons (LK.verum Γ ∅)
+  falsum := wkL (by simp) (LK.falsum ∅ ∅)
+  negLeft {Γ A} (d) := LK.negLeft (ofSingleton d)
+  negRight {Γ A} (d) := ofCons <| LK.negRight d
+  andLeft₁ {Γ A B C} (d) := ofCons <| LK.andLeft <| wkL (Precollection.subset_iff.mpr <| by aesop) (ofSingleton d)
+  andLeft₂ {Γ A B C} (d) := ofCons <| LK.andLeft <| wkL (Precollection.subset_iff.mpr <| by aesop) (ofSingleton d)
+  andRight {Γ A B} (dA dB) := ofCons <| LK.andRight (ofSingleton dA) (ofSingleton dB)
+  orLeft {Γ A B C} (dA dB) := ofCons <| LK.orLeft (ofSingleton dA) (ofSingleton dB)
+  orRight₁ {Γ A B} (d) := ofCons <| LK.orRight <| wkR (Precollection.subset_iff.mpr <| by aesop) (ofSingleton d)
+  orRight₂ {Γ A B} (d) := ofCons <| LK.orRight <| wkR (Precollection.subset_iff.mpr <| by aesop) (ofSingleton d)
+  implyLeft {Γ A B C} (dA dB) := ofCons <| LK.implyLeft
+    (wkR (Precollection.subset_iff.mpr <| by aesop) (ofSingleton dA))
+    (ofSingleton dB)
+  implyRight {Γ A B} (d) := ofCons <| LK.implyRight <| ofSingleton d
+
+end LK
+
+end TwosidedCalc
